CyclicBuffer: try transitions that more closely resemble tokens

concurrency/node-replication/CyclicBuffer.i.dfy
@@ -1,38 +1,38 @@
+include "Constants.i.dfy"
 include "../../lib/Lang/NativeTypes.s.dfy"
 include "InfiniteLogTokens.i.dfy"
 include "../framework/Cells.s.dfy"
+include "../framework/MultiRw.i.dfy"
 include "../framework/GlinearOption.s.dfy"
-include "Constants.i.dfy"
+include "../../lib/Base/Option.s.dfy"
 
 
 module CyclicBufferRw(nrifc: NRIfc) refines MultiRw {
+  import IL = InfiniteLogSSM(nrifc)
+  import opened ILT = InfiniteLogTokens(nrifc)
+  import opened GlinearOption
+  import opened Cells
+  import opened Options
+  import opened Constants
+
   type Key(!new) = nat
 
   glinear datatype StoredType = StoredType(
-    glinear cellContents: CellContents<LogEntry>,
-    glinear logEntry: glOption<Log>
+    glinear cellContents: CellContents<IL.LogEntry>,
+    glinear logEntry: glOption<ILT.Log>
   )
 
-  datatype AdvanceHeadState =
-    | AdvanceHeadIdle
-    | AdvHeadNextLoaded(next: NodeId)
-    | AdvHeadHeadLoaded(next: NodeId, head : nat)
-    | AdvHeadMinLtail(next: NodeId, head: nat, mintail: nat, idx: NodeId)
-
-  // not sure fi that one s needed?
-  //datatype AdvanceTailState = AdvanceTailState(obvserve_head: nat)
-
-  datatype AppendState =
-    | AppendIdle
-    | AppendAdvanceTail(ops: seq<nrifc.UpdateOp>, tail: nat)
-    | AppendWriteLogEntry(ops: seq<nrifc.UpdateOp>, tail: nat, idx: nat)
-
-
   datatype ReaderState =
-    | ReaderIdle
-    | ReaderLoadTail(ltail: nat)
-    | ReaderReadEntries(ltail: nat, gtail:nat)
+    | ReaderStarting(ghost start: nat)
+    | ReaderRange(ghost start: nat, ghost end: nat)
+    | ReaderGuard(ghost start: nat, ghost end: nat, ghost cur: nat, ghost val: StoredType)
 
+  datatype CombinerState =
+    | CombinerIdle
+    | CombinerReading(ghost readerState: ReaderState)
+    | CombinerAdvancingHead(ghost idx: nat, ghost min_tail: nat)
+    | CombinerAdvancingTail(ghost obvserve_head: nat)
+    | CombinerAppendState(ghost cur_idx: nat, ghost tail: nat)
 
   // define the nodeid type
   type NodeId = nat
@@ -47,40 +47,20 @@ module CyclicBufferRw(nrifc: NRIfc) refines MultiRw {
       // New appends go here.
       tail: Option<nat>,
 
-      // Completed tail maintains an index <= tail that points to a
-      // log entry after which there are no completed operations across
-      // all replicas registered against this log.
-      // TODO(RA): do we need this?
-      // ctail: Option<nat>,
-
       // Array consisting of the local tail of each replica registered with the log.
       // Required for garbage collection; since replicas make progress over the log
       // independently, we want to make sure that we don't garbage collect operations
       // that haven't been executed by all replicas.
-      ltails: map<NodeId, nat>,
+      localTails: map<NodeId, nat>,
 
-      // Identifier that will be allocated to the next replica that registers with
-      // this Log. Also required to correctly index into ltails above.
-      next: Option<NodeId>,
+      contents: map<int, StoredType>,
 
-      /// Array consisting of local alive masks for each registered replica. Required
-      /// because replicas make independent progress over the log, so we need to
-      /// track log wrap-arounds for each of them separately.
-      lmasks: map<NodeId, bool>,
+      // The 'alive' bit flips back and forth. So sometimes 'true' means 'alive',
+      // and sometimes 'false' means 'alive'.
+      // entry is an index into the buffer (0 <= entry < BUFFER_SIZE)
+      aliveBits: map</* entry: */ nat, /* bit: */ bool>,
 
-      /// The maximum number of entries that can be held inside the log.
-      size: Option<nat>,
-
-      /// A reference to the actual log. Nothing but a slice of entries.
-      // slog: &'a [Cell<Entry<T>>],
-      slog: map<int, StoredType>,
-
-
-      // TODO: could we have multiple threads advancing the head, we assume so
-      advanceHead: map<NodeId, AdvanceHeadState>,
-      // advanceTail: map<NodeId, AdvanceTailState>,
-      readerState: map<NodeId, ReaderState>,
-      appendState: map<NodeId, AppendState>
+      combinerState: map<NodeId, CombinerState>
     )
 
   function dot(x: M, y: M) : M
@@ -88,564 +68,641 @@ module CyclicBufferRw(nrifc: NRIfc) refines MultiRw {
 
   predicate Init(s: M)
   predicate Inv(x: M)
-  function I(x: M) : map<Key, StoredType> requires Inv(x)
+  function I(x: M) : map<Key, StoredType>
+
+  /*
+   * ============================================================================================
+   * Buffer Utilities
+   * ============================================================================================
+   */
+
+  function Index(logical: int) : nat
+  // ensures Index(-(BUFFER_SIZE as int)) == 0
+  {
+    logical % (BUFFER_SIZE as int)
+  }
+
+  /*
+   * ============================================================================================
+   * State Guards
+   * ============================================================================================
+   */
+
+  predicate LocalTailValid(m: M, nodeId: NodeId)
+    requires m.M?
+  {
+    && nodeId in m.localTails
+  }
+
+  predicate CombierIdle(m: M, nodeId: NodeId)
+    requires m.M?
+  {
+    && nodeId in m.combinerState
+    && m.combinerState[nodeId] == CombinerIdle
+  }
+
+  predicate CombinerKnown(m: M, nodeId: NodeId)
+    requires m.M?
+  {
+    && nodeId in m.combinerState
+  }
+
+  predicate CombinerIsAdvancingHead(m: M, nodeId: NodeId)
+    requires m.M?
+    requires CombinerKnown(m, nodeId)
+  {
+    && m.combinerState[nodeId].CombinerAdvancingHead?
+  }
+
+  predicate CombinerIsAdvancingHeadAt(m: M, nodeId: NodeId, idx: nat, min_tail: nat)
+    requires m.M?
+    requires CombinerKnown(m, nodeId)
+  {
+    && m.combinerState[nodeId] == CombinerAdvancingHead(idx, min_tail)
+  }
+
+  /*
+   * ============================================================================================
+   * Advance Head Transitions
+   * ============================================================================================
+   */
+
+  predicate InitAdvanceHead(m: M, m': M, combinerNodeId: nat)
+  {
+    && m.M?
+    && LocalTailValid(m, 0)
+
+    && m'.M?
+    && CombinerKnown(m', combinerNodeId)
+    && CombinerIsAdvancingHeadAt(m', combinerNodeId, 1, m.localTails[0])
+  }
+
+  predicate StepAdvanceHead(m: M, m': M, combinerNodeId: nat)
+  {
+    && m.M?
+    && CombinerKnown(m, combinerNodeId)
+    && CombinerIsAdvancingHead(m, combinerNodeId)
+    && var combinerBefore := m.combinerState[combinerNodeId];
+    && LocalTailValid(m, combinerBefore.idx)
+
+    && m'.M?
+    && CombinerKnown(m', combinerNodeId)
+    && CombinerIsAdvancingHeadAt(m', combinerNodeId, combinerBefore.idx + 1,
+      if combinerBefore.min_tail < m.localTails[combinerBefore.idx]
+        then combinerBefore.min_tail
+        else m.localTails[combinerBefore.idx])
+  }
+
+  predicate FinishAdvanceHead(m: M, m': M, combinerNodeId: nat)
+  {
+    && m.M?
+    && CombinerKnown(m, combinerNodeId)
+    && CombinerIsAdvancingHead(m, combinerNodeId)
+    && var combinerBefore := m.combinerState[combinerNodeId];
+    && combinerBefore.idx == (NUM_REPLICAS as nat)
+
+    && m'.M?
+    && m'.head.Some?
+    && m'.head.value == combinerBefore.min_tail
+  }
+
+  /*
+   * ============================================================================================
+   * Advance Tail Transitions
+   * ============================================================================================
+   */
+
+  // predicate InitAdvanceTail(m: M, m': M, advancerNodeId: nat)
+  // {
+  //   && m.M?
+  //   && 
+  // }
 
   /////////////////////////////////////////////////////////////////////////////
   // Functions
   /////////////////////////////////////////////////////////////////////////////
 
-  function Index(idx: nat, size: nat) : nat {
-    // logical & (self.size - 1)
-    idx % size
-  }
-
-  /////////////////////////////////////////////////////////////////////////////
-  // State Guards
-  /////////////////////////////////////////////////////////////////////////////
-
-  predicate StateValid(m: M) {
-    m.M?
-  }
-
-  predicate NextFieldValid(m: M)
-    requires StateValid(m)
-  {
-    m.next.Some?
-  }
-
-  predicate HeadFieldValid(m: M)
-    requires StateValid(m)
-  {
-    m.head.Some?
-  }
-
-  predicate TailFieldValid(m: M)
-    requires StateValid(m)
-  {
-    m.tail.Some?
-  }
-
-  /////////////////////////////////////////////////////////////////////////////
-  // Advance Head Guards
-  /////////////////////////////////////////////////////////////////////////////
-
-  // we're in the advance head idle state
-  predicate AdvHeadInIdle(m: M, nodeId: NodeId)
-    requires StateValid(m)
-  {
-    && nodeId in m.advanceHead
-    && m.advanceHead[nodeId].AdvanceHeadIdle?
-  }
-
-  predicate AdvHeadInNextLoaded(m: M, nodeId: NodeId)
-    requires StateValid(m)
-  {
-    && nodeId in m.advanceHead
-    && m.advanceHead[nodeId].AdvHeadNextLoaded?
-  }
-
-  predicate AdvHeadInReadHead(m: M, nodeId: NodeId)
-    requires StateValid(m)
-  {
-    && nodeId in m.advanceHead
-    && m.advanceHead[nodeId].AdvHeadHeadLoaded?
-  }
-
-  predicate AdvHeadInMinLTail(m: M, nodeId: NodeId)
-    requires StateValid(m)
-  {
-    && nodeId in m.advanceHead
-    && m.advanceHead[nodeId].AdvHeadMinLtail?
-    && m.advanceHead[nodeId].idx < m.advanceHead[nodeId].next
-  }
-
-  predicate AdvHeadMinLtailValid(m: M, nodeId: NodeId)
-    requires AdvHeadInMinLTail(m, nodeId)
-  {
-    && var st := m.advanceHead[nodeId];
-    && st.idx in m.LocalTails
-  }
-
-  predicate AdvHeadInMinLTailDone(m: M, nodeId: NodeId)
-    requires StateValid(m)
-  {
-    && nodeId in m.advanceHead
-    && m.advanceHead[nodeId].AdvHeadMinLtail?
-    && m.advanceHead[nodeId].idx == m.advanceHead[nodeId].next
-  }
-
-  /////////////////////////////////////////////////////////////////////////////
-  // Append Guards
-  /////////////////////////////////////////////////////////////////////////////
-
-  predicate AppendInIdle(m: M, nodeId: NodeId)
-    requires StateValid(m)
-  {
-    && nodeId in m.appendState
-    && m.appendState[nodeId].AppendIdle?
-  }
-
-  predicate AppendInAdvanceTail(m: M, nodeId: NodeId)
-    requires StateValid(m)
-  {
-    && nodeId in m.appendState
-    && m.appendState[nodeId].AppendAdvanceTail?
-  }
-
-  predicate AppendInWriteLogEntryFlipMask(m: M, nodeId: NodeId)
-    requires StateValid(m)
-  {
-    && nodeId in m.appendState
-    && m.appendState[nodeId].AppendWriteLogEntry?
-    && m.appendState[nodeId].idx < |m.appendState[nodeId].ops|
-    && nodeId in m.lmasks
-    && st.idx in m.slog
-    && m.slog[st.idx].alive == m.lmasks[nodeId]
-  }
-
-  predicate AppendInWriteLogEntryDone(m: M, nodeId: NodeId)
-    requires StateValid(m)
-  {
-    && nodeId in m.appendState
-    && m.appendState[nodeId].AppendWriteLogEntry?
-    && m.appendState[nodeId].idx == |m.appendState[nodeId].ops|
-  }
-
-  predicate AppendInWriteLogEntry(m: M, nodeId: NodeId)
-    requires StateValid(m)
-  {
-    && nodeId in m.appendState
-    && m.appendState[nodeId].AppendWriteLogEntry?
-    && nodeId in m.lmasks
-    && st.idx in m.slog
-    && m.slog[st.idx].alive != m.lmasks[nodeId]
-  }
-
-
-  /////////////////////////////////////////////////////////////////////////////
-  // Reader Guards
-  /////////////////////////////////////////////////////////////////////////////
-
-  predicate ReaderInIdle(m: M, nodeId: NodeId)
-    requires StateValid(m)
-  {
-    && nodeId in m.readerState
-    && m.readerState[nodeId].ReaderIdle?
-  }
-
-  predicate ReaderInLoadTail(m: M, nodeId: NodeId)
-    requires StateValid(m)
-  {
-    && nodeId in m.readerState
-    && m.readerState[nodeId].ReaderLoadTail?
-  }
-
-  predicate ReaderInReadEntries(m: M, nodeId: NodeId)
-    requires StateValid(m)
-  {
-    && nodeId in m.readerState
-    && m.readerState[nodeId].ReaderReadEntries?
-    && m.readerState[nodeId].ltail != m.readerState[nodeId].gtail
-  }
-
-  predicate ReaderInReadEntriesDone(m: M, nodeId: NodeId)
-    requires StateValid(m)
-  {
-    && nodeId in m.readerState
-    && nodeId in m.localTails
-    && m.readerState[nodeId].ReaderReadEntries?
-    && m.readerState[nodeId].ltail == m.readerState[nodeId].gtail
-    && m.readerState[nodeId].ltail != m.localTails[nodeId]
-  }
-
-  predicate ReaderInReadEntriesDoneNoUpdate(m: M, nodeId: NodeId)
-    requires StateValid(m)
-  {
-    && nodeId in m.readerState
-    && nodeId in m.localTails
-    && m.readerState[nodeId].ReaderReadEntries?
-    && m.readerState[nodeId].ltail == m.readerState[nodeId].gtail
-    && m.readerState[nodeId].ltail == m.localTails[nodeId]
-  }
-
-  /////////////////////////////////////////////////////////////////////////////
-  // Reading Transitions
-  /////////////////////////////////////////////////////////////////////////////
-
-  // { ReaderIdle }
-  //   let ltail = self.ltails[idx - 1].load(Ordering::Relaxed);
-  // { ReaderLoadTail(ltail) }
-  predicate TransitionReaderLoadTail(m: M, m': M, nodeId: NodeId)
-  {
-    && StateValid(m)
-    && ReaderInIdle(m, nodeId)
-
-    // get the local tail
-    && var ltail := m.localTails[nodeId];
-
-    // construct the new state
-    && var new_st := ReaderLoadTail(ltail);
-
-    // the state transition
-    && m' == m.(readerState := m.readerState[ nodeId := new_st ])
-  }
-
-
-  // { ReaderLoadTail(ltail) }
-  //   let gtail = self.tail.load(Ordering::Relaxed);
-  // { ReaderReadEntries(ltail, gtail) }
-  predicate TransitionReaderReadEntries(m: M, m': M, nodeId: NodeId)
-  {
-    && StateValid(m)
-    && ReaderInLoadTail(m, nodeId)
-
-    // the old state
-    && var st := m.readerState[nodeId];
-
-    // get the local tail
-    && var gtail := m.tail.value;
-
-    // construct the new state
-    && var new_st := ReaderReadEntries(ltail, gtail);
-
-    // the state transition
-    && m' == m.(readerState := m.readerState[ nodeId := new_st ])
-  }
-
-  // { ReaderReadEntries(ltail, gtail) }
-  // { (*e).alivef.load(Ordering::Acquire) == self.lmasks[idx - 1].get() }
-  //   d((*e).operation.as_ref().unwrap().clone(), (*e).replica)
-  //   if self.index(i) == self.size - 1 { self.lmasks[idx - 1].set(!self.lmasks[idx - 1].get()); }
-  // { ReaderReadEntries(ltail + 1, gtail)  }
-  predicate TransitionReaderReadEntry(m: M, m': M, nodeId: NodeId)
-  {
-    && StateValid(m)
-    && ReaderInReadEntries(m, nodeId)
-
-    // the old state
-    && var st := m.readerState[nodeId];
-
-    && var entry := m.slog[st.ltail];
-    // TODO: do something
-
-    // update the new lmask if needed
-    && var m := m.lmasks[nodeId];
-    && var new_mask := if Index(st.ltail, m.size) == m.size - 1 then !m else m;
-
-    // construct the new state
-    && var new_st := ReaderReadEntries(st.ltail + 1, st.gtail);
-
-    // the state transition
-    && m' == m.(readerState := m.readerState[ nodeId := new_st ])
-              .(lmasks := m.lmasks[nodeId := new_mask])
-
-  }
-
-
-  // { ReaderReadEntries(ltail, gtail)}
-  // { gtail == ltail } && { m.localTails[nodeId] == ltail }
-  //   if ltail == gtail { return; }
-  // { ReaderIdle }
-  predicate TransitionReaderIdleNoUpdates(m: M, m': M, nodeId: NodeId)
-  {
-    && StateValid(m)
-    && ReaderInReadEntriesDoneNoUpdate(m, nodeId)
-
-    // construct the new state
-    && var new_st := ReaderIdle;
-
-    // the state transition
-    && m' == m.(readerState := m.readerState[ nodeId := new_st ])
-  }
-
-
-
-  // { ReaderReadEntries(ltail, gtail)}
-  // { gtail == ltail } && { m.localTails[nodeId] != ltail }
-  //    self.ltails[idx - 1].store(gtail, Ordering::Relaxed);
-  // { ReaderIdle }
- predicate ReaderInReadEntriesDone(m: M, m': M, nodeId: NodeId)
-  {
-    && StateValid(m)
-    && ReaderInReadEntries(m, nodeId)
-
-    // the old state
-    && var st := m.readerState[nodeId];
-
-    // get the local tail
-    && var gtail := m.tail.value;
-
-    // construct the new state
-    && var new_st := ReaderIdle;
-
-    // the new ltail si the gtail
-    && var new_ltail := st.gtail;
-
-    // the state transition
-    && m' == m.(readerState := m.readerState[ nodeId := new_st ])
-              .(ltails := m.ltails[nodeId := new_ltail])
-  }
-
-
-
-  /////////////////////////////////////////////////////////////////////////////
-  // Append Transitions
-  /////////////////////////////////////////////////////////////////////////////
-
-  // pub fn append<F: FnMut(T, usize)>(&self, ops: &[T], idx: usize, mut s: F)
-
-
-  // { AppendIdle }
-  //   let tail = self.tail.load(Ordering::Relaxed);
-  // { AppendAdvanceTail(ops, tail) }
-  predicate TransitionAppendAdvanceTail(m: M, m': M, nodeId: NodeId, ops: seq<nrifc.UpdateOp>) {
-      && StateValid(m)
-      && AppendInIdle(m, nodeId)
-      && TailFieldValid(m)
-
-      // read the tail field
-      && var tail := m.tail.value;
-
-      // construct the new state
-      && var newst := AppendAdvanceTail(ops, tail);
-
-      // the state transition
-      && m' == m.(appendState := m.appendState[nodeId := newst])
-  }
-  // TODO, the case where we exec??? if tail > head + self.size - GC_FROM_HEAD {
-
-  // { AppendAdvanceTail(ops, tail) }
-  // self.tail.compare_exchange_weak()  // if we had another update
-  // { AppendAdvanceTail(ops, tail) }
-  predicate TransitionAppendWriteLogEntry(m: M, m': M, nodeId: NodeId) {
-      && StateValid(m)
-      && AppendAdvanceTail(m, nodeId)
-      && TailFieldValid(m)
-
-      // read the tail field
-      && var tail := m.tail.value;
-
-      // the old state
-      var st := m.appendState[nodeId];
-
-      // if the two tails are not equal, retry
-      && st.tail != tail
-
-      // construct the new state
-      && var newst := AppendAdvanceTail(ops, tail);
-
-      // the state transition
-      && m' == m.(appendState := m.appendState[nodeId := newst])
-  }
-
-
-  // { AppendAdvanceTail(ops, tail) }
-  // self.tail.compare_exchange_weak()
-  // { AppendWriteLogEntry(ops, tail, idx = 0) }
-  predicate TransitionAppendWriteLogEntry(m: M, m': M, nodeId: NodeId) {
-      && StateValid(m)
-      && AppendInAdvanceTail(m, nodeId)
-      && TailFieldValid(m)
-
-      // read the tail field
-      && var tail := m.tail.value;
-
-      // the old state
-      var st := m.appendState[nodeId];
-
-      // the two tails must be equal
-      && st.tail == tail
-
-      // read the tail field
-      && var tail_new := tail + |st.ops|;
-
-      // construct the new state
-      && var newst := AppendWriteLogEntry(ops, tail, idx);
-
-      // the state transition
-      && m' == m.(appendState := m.appendState[nodeId := newst])
-                .(tail := Some(tail_new))
-  }
-
-  // { AppendWriteLogEntry(ops, tail, idx) }
-  //   if unsafe { (*e).alivef.load(Ordering::Relaxed) == m } { m = !m; }
-  // { AppendWriteLogEntry(ops, tail, idx) }
-  predicate TransitionAppendWriteLogEntryOp(m: M, m': M, nodeId: NodeId) {
-      && StateValid(m)
-      && AppendInWriteLogEntryFlipMask(m, nodeId)
-
-      // the old state
-      && var st := m.appendState[nodeId];
-
-      // construct the new state
-      && var newst := AppendWriteLogEntryOp(ops, tail, idx);
-
-      // construct the new mask value
-      && var newmask := !m.lmasks[nodeId];
-
-      // the state transition
-      && m' == m.(appendState := m.appendState[nodeId := newst])
-                .(lmasks := m.lmasks[nodeId := newmask])
-  }
-
-  // { AppendWriteLogEntry(ops, tail, idx) }
-  //   unsafe { (*e).alivef.store(m, Ordering::Release) };
-  // { AppendWriteLogEntry(ops, tail, idx + 1) }
-  predicate TransitionAppendWriteLogNext(m: M, m': M, nodeId: NodeId) {
-      && StateValid(m)
-      && AppendInWriteLogEntry(m, nodeId)
-
-      // the old state
-      && var st := m.appendState[nodeId];
-
-      // construct the new state
-      && var newst := AppendWriteLogEntryOp(ops, tail, idx + 1);
-
-      // construct the log entry
-      && var logentry := StoredType(st.ops[st.idx]);
-
-      // the state transition
-      && m' == m.(appendState := m.appendState[nodeId := newst])
-                .(slog := m.slog[st.tail + st.idx := logentry])
-  }
-
-  // assert idx == |ops|
-  // { AppendWriteLogEntry(ops, tail, idx + 1) }
-  // { AppendIdle }
-  predicate TransitionAppendWriteLogDone(m: M, m': M, nodeId: NodeId) {
-      && StateValid(m)
-      && AppendInWriteLogEntryDone(m, nodeId)
-
-      // construct the new state
-      && var newst := AppendIdle;
-
-       // the state transition
-      && m' == m.(appendState := m.appendState[nodeId := newst])
-  }
-
-
-
-  /////////////////////////////////////////////////////////////////////////////
-  // AdvanceHead Transitions
-  /////////////////////////////////////////////////////////////////////////////
-
-  // fn advance_head<F: FnMut(T, usize)>(&self, rid: usize, mut s: &mut F);
-
-  // { AdvHeadIdle }
-  //   let r = self.next.load(Ordering::Relaxed);
-  // { AdvHeadNextLoaded(next) }
-  predicate TransitionAdvHeadLoadNext(m: M, m': M, nodeId: NodeId) {
-    && StateValid(m)
-    && AdvHeadInIdle(m, nodeId)
-    && NextFieldValid(m)
-
-    // read the next field
-    && var next := m.next.value;
-
-    // construct the new state
-    && var newst := AdvHeadNextLoaded(next);
-
-    // update the state of the advanceHead
-    && m' == m.(advanceHead := m.advanceHead[ nodeId :=  newst])
-  }
-
-  // { AdvHeadNextLoaded(next) }
-  //   let global_head = self.head.load(Ordering::Relaxed);
-  // { AdvHeadHeadLoaded(next, head) }
-  predicate TransitionAdvHeadReadHead(m: M, m': M, nodeId: NodeId) {
-    && StateValid(m)
-    && AdvHeadInNextLoaded(m, nodeId)
-    && HeadFieldValid(m)
-
-    // get the old state
-    && var st := m.advanceHead[nodeId];
-
-    // read the next field
-    && var head := m.head.value;
-
-    // construct the new state
-    && var newst := AdvHeadNextLoaded(st.next, head);
-
-    // update the state of the advanceHead
-    && m' == m.(advanceHead := m.advanceHead[ nodeId :=  newst])
-  }
-
-
-  // let f = self.tail.load(Ordering::Relaxed);
-  // that one seems to be no-where used??
-
-  // { AdvHeadHeadLoaded(next, head) }
-  //   let mut min_local_tail = self.ltails[0].load(Ordering::Relaxed);
-  // { AdvHeadMinLtail(next, head, min_local_tail, idx = 1) }
-  predicate TransitionAdvHeadMinLTail(m: M, m': M, nodeId: NodeId) {
-    && StateValid(m)
-    && AdvHeadInReadHead(m, nodeId)
-    && 0 in m.localTails
-
-    // get the old state
-    && var st := m.advanceHead[nodeId];
-
-    // read the first local tail
-    && var ltail := m.localTails[0];
-
-    // construct the new state
-    && var newst := AdvHeadMinLtail(st.next, st.head, ltail, 1);
-
-    // update the state of the advanceHead
-    && m' == m.(advanceHead := m.advanceHead[ nodeId :=  newst])
-  }
-
-
-  // { AdvHeadMinLtail(next, head, min_local_tail, idx = 1)
-  //   for idx in 1..r {
-  //     let cur_local_tail = self.ltails[idx - 1].load(Ordering::Relaxed);
-  //     if min_local_tail > cur_local_tail {
-  //         min_local_tail = cur_local_tail
-  //     };
-  //   }
-  // assert(idx == next)
-  // { AdvHeadMinLtail(next, head, min_local_tail, idx = next)
-  predicate TransitionAdvHeadMinLTailNext(m: M, m': M, nodeId: NodeId) {
-    && StateValid(m)
-    && AdvHeadInMinLTail(m, nodeId)
-    && AdvHeadMinLtailValid(m, nodeId)
-
-    // get the old state
-    && var st := m.advanceHead[nodeId];
-
-    // read the current local tail
-    && var cur_local_tail := m.localTails[st.idx];
-
-    // if the current local tail is smaller, update the value
-    && var ltail := if st.mintail > cur_local_tail then cur_local_tail else st.mintail;
-
-    // construct the new state
-    && var newst := AdvHeadMinLtail(st.next, st.head, ltail, st.idx + 1);
-
-    // update the state of the advanceHead
-    && m' == m.(advanceHead := m.advanceHead[ nodeId :=  newst])
-  }
-
-  // What About the exec stuff here?
-  // { AdvHeadMinLtail(next, head, min_local_tail, idx = next)
-  //   self.head.store(min_local_tail, Ordering::Relaxed);
-  // { AdvHeadIdle }
-  predicate TransitionAdvHeadIdle(m: M, m': M, nodeId: NodeId) {
-    && StateValid(m)
-    && AdvHeadInMinLTailDone(m, nodeId)
-
-    // get the old state
-    && var st := m.advanceHead[nodeId];
-
-    // the new head value
-    && var new_head := st.mintail;
-
-    // construct the new state
-    && var newst := AdvHeadIdle;
-
-    // update the state of the advanceHead
-    && m' == m.(advanceHead := m.advanceHead[ nodeId :=  newst])
-              .(head := Some(new_head))
-  }
+  // /////////////////////////////////////////////////////////////////////////////
+  // // Advance Head Guards
+  // /////////////////////////////////////////////////////////////////////////////
+
+  // // we're in the advance head idle state
+  // predicate AdvHeadInIdle(m: M, nodeId: NodeId)
+  //   requires StateValid(m)
+  // {
+  //   && nodeId in m.advanceHead
+  //   && m.advanceHead[nodeId].AdvanceHeadIdle?
+  // }
+
+  // predicate AdvHeadInNextLoaded(m: M, nodeId: NodeId)
+  //   requires StateValid(m)
+  // {
+  //   && nodeId in m.advanceHead
+  //   && m.advanceHead[nodeId].AdvHeadNextLoaded?
+  // }
+
+  // predicate AdvHeadInReadHead(m: M, nodeId: NodeId)
+  //   requires StateValid(m)
+  // {
+  //   && nodeId in m.advanceHead
+  //   && m.advanceHead[nodeId].AdvHeadHeadLoaded?
+  // }
+
+  // predicate AdvHeadInMinLTail(m: M, nodeId: NodeId)
+  //   requires StateValid(m)
+  // {
+  //   && nodeId in m.advanceHead
+  //   && m.advanceHead[nodeId].AdvHeadMinLtail?
+  //   && m.advanceHead[nodeId].idx < m.advanceHead[nodeId].next
+  // }
+
+  // predicate AdvHeadMinLtailValid(m: M, nodeId: NodeId)
+  //   requires AdvHeadInMinLTail(m, nodeId)
+  // {
+  //   && var st := m.advanceHead[nodeId];
+  //   && st.idx in m.LocalTails
+  // }
+
+  // predicate AdvHeadInMinLTailDone(m: M, nodeId: NodeId)
+  //   requires StateValid(m)
+  // {
+  //   && nodeId in m.advanceHead
+  //   && m.advanceHead[nodeId].AdvHeadMinLtail?
+  //   && m.advanceHead[nodeId].idx == m.advanceHead[nodeId].next
+  // }
+
+  // /////////////////////////////////////////////////////////////////////////////
+  // // Append Guards
+  // /////////////////////////////////////////////////////////////////////////////
+
+  // predicate AppendInIdle(m: M, nodeId: NodeId)
+  //   requires StateValid(m)
+  // {
+  //   && nodeId in m.appendState
+  //   && m.appendState[nodeId].AppendIdle?
+  // }
+
+  // predicate AppendInAdvanceTail(m: M, nodeId: NodeId)
+  //   requires StateValid(m)
+  // {
+  //   && nodeId in m.appendState
+  //   && m.appendState[nodeId].AppendAdvanceTail?
+  // }
+
+  // predicate AppendInWriteLogEntryFlipMask(m: M, nodeId: NodeId)
+  //   requires StateValid(m)
+  // {
+  //   && nodeId in m.appendState
+  //   && m.appendState[nodeId].AppendWriteLogEntry?
+  //   && m.appendState[nodeId].idx < |m.appendState[nodeId].ops|
+  //   && nodeId in m.lmasks
+  //   && st.idx in m.slog
+  //   && m.slog[st.idx].alive == m.lmasks[nodeId]
+  // }
+
+  // predicate AppendInWriteLogEntryDone(m: M, nodeId: NodeId)
+  //   requires StateValid(m)
+  // {
+  //   && nodeId in m.appendState
+  //   && m.appendState[nodeId].AppendWriteLogEntry?
+  //   && m.appendState[nodeId].idx == |m.appendState[nodeId].ops|
+  // }
+
+  // predicate AppendInWriteLogEntry(m: M, nodeId: NodeId)
+  //   requires StateValid(m)
+  // {
+  //   && nodeId in m.appendState
+  //   && m.appendState[nodeId].AppendWriteLogEntry?
+  //   && nodeId in m.lmasks
+  //   && st.idx in m.slog
+  //   && m.slog[st.idx].alive != m.lmasks[nodeId]
+  // }
+
+
+  // /////////////////////////////////////////////////////////////////////////////
+  // // Reader Guards
+  // /////////////////////////////////////////////////////////////////////////////
+
+  // predicate ReaderInIdle(m: M, nodeId: NodeId)
+  //   requires StateValid(m)
+  // {
+  //   && nodeId in m.readerState
+  //   && m.readerState[nodeId].ReaderIdle?
+  // }
+
+  // predicate ReaderInLoadTail(m: M, nodeId: NodeId)
+  //   requires StateValid(m)
+  // {
+  //   && nodeId in m.readerState
+  //   && m.readerState[nodeId].ReaderLoadTail?
+  // }
+
+  // predicate ReaderInReadEntries(m: M, nodeId: NodeId)
+  //   requires StateValid(m)
+  // {
+  //   && nodeId in m.readerState
+  //   && m.readerState[nodeId].ReaderReadEntries?
+  //   && m.readerState[nodeId].ltail != m.readerState[nodeId].gtail
+  // }
+
+  // predicate ReaderInReadEntriesDone(m: M, nodeId: NodeId)
+  //   requires StateValid(m)
+  // {
+  //   && nodeId in m.readerState
+  //   && nodeId in m.localTails
+  //   && m.readerState[nodeId].ReaderReadEntries?
+  //   && m.readerState[nodeId].ltail == m.readerState[nodeId].gtail
+  //   && m.readerState[nodeId].ltail != m.localTails[nodeId]
+  // }
+
+  // predicate ReaderInReadEntriesDoneNoUpdate(m: M, nodeId: NodeId)
+  //   requires StateValid(m)
+  // {
+  //   && nodeId in m.readerState
+  //   && nodeId in m.localTails
+  //   && m.readerState[nodeId].ReaderReadEntries?
+  //   && m.readerState[nodeId].ltail == m.readerState[nodeId].gtail
+  //   && m.readerState[nodeId].ltail == m.localTails[nodeId]
+  // }
+
+  // /////////////////////////////////////////////////////////////////////////////
+  // // Reading Transitions
+  // /////////////////////////////////////////////////////////////////////////////
+
+  // // { ReaderIdle }
+  // //   let ltail = self.ltails[idx - 1].load(Ordering::Relaxed);
+  // // { ReaderLoadTail(ltail) }
+  // predicate TransitionReaderLoadTail(m: M, m': M, nodeId: NodeId)
+  // {
+  //   && StateValid(m)
+  //   && ReaderInIdle(m, nodeId)
+
+  //   // get the local tail
+  //   && var ltail := m.localTails[nodeId];
+
+  //   // construct the new state
+  //   && var new_st := ReaderLoadTail(ltail);
+
+  //   // the state transition
+  //   && m' == m.(readerState := m.readerState[ nodeId := new_st ])
+  // }
+
+
+  // // { ReaderLoadTail(ltail) }
+  // //   let gtail = self.tail.load(Ordering::Relaxed);
+  // // { ReaderReadEntries(ltail, gtail) }
+  // predicate TransitionReaderReadEntries(m: M, m': M, nodeId: NodeId)
+  // {
+  //   && StateValid(m)
+  //   && ReaderInLoadTail(m, nodeId)
+
+  //   // the old state
+  //   && var st := m.readerState[nodeId];
+
+  //   // get the local tail
+  //   && var gtail := m.tail.value;
+
+  //   // construct the new state
+  //   && var new_st := ReaderReadEntries(ltail, gtail);
+
+  //   // the state transition
+  //   && m' == m.(readerState := m.readerState[ nodeId := new_st ])
+  // }
+
+  // // { ReaderReadEntries(ltail, gtail) }
+  // // { (*e).alivef.load(Ordering::Acquire) == self.lmasks[idx - 1].get() }
+  // //   d((*e).operation.as_ref().unwrap().clone(), (*e).replica)
+  // //   if self.index(i) == self.size - 1 { self.lmasks[idx - 1].set(!self.lmasks[idx - 1].get()); }
+  // // { ReaderReadEntries(ltail + 1, gtail)  }
+  // predicate TransitionReaderReadEntry(m: M, m': M, nodeId: NodeId)
+  // {
+  //   && StateValid(m)
+  //   && ReaderInReadEntries(m, nodeId)
+
+  //   // the old state
+  //   && var st := m.readerState[nodeId];
+
+  //   && var entry := m.slog[st.ltail];
+  //   // TODO: do something
+
+  //   // update the new lmask if needed
+  //   && var m := m.lmasks[nodeId];
+  //   && var new_mask := if Index(st.ltail, m.size) == m.size - 1 then !m else m;
+
+  //   // construct the new state
+  //   && var new_st := ReaderReadEntries(st.ltail + 1, st.gtail);
+
+  //   // the state transition
+  //   && m' == m.(readerState := m.readerState[ nodeId := new_st ])
+  //             .(lmasks := m.lmasks[nodeId := new_mask])
+
+  // }
+
+
+  // // { ReaderReadEntries(ltail, gtail)}
+  // // { gtail == ltail } && { m.localTails[nodeId] == ltail }
+  // //   if ltail == gtail { return; }
+  // // { ReaderIdle }
+  // predicate TransitionReaderIdleNoUpdates(m: M, m': M, nodeId: NodeId)
+  // {
+  //   && StateValid(m)
+  //   && ReaderInReadEntriesDoneNoUpdate(m, nodeId)
+
+  //   // construct the new state
+  //   && var new_st := ReaderIdle;
+
+  //   // the state transition
+  //   && m' == m.(readerState := m.readerState[ nodeId := new_st ])
+  // }
+
+
+
+  // // { ReaderReadEntries(ltail, gtail)}
+  // // { gtail == ltail } && { m.localTails[nodeId] != ltail }
+  // //    self.ltails[idx - 1].store(gtail, Ordering::Relaxed);
+  // // { ReaderIdle }
+  // redicate ReaderInReadEntriesDone(m: M, m': M, nodeId: NodeId)
+  // {
+  //   && StateValid(m)
+  //   && ReaderInReadEntries(m, nodeId)
+
+  //   // the old state
+  //   && var st := m.readerState[nodeId];
+
+  //   // get the local tail
+  //   && var gtail := m.tail.value;
+
+  //   // construct the new state
+  //   && var new_st := ReaderIdle;
+
+  //   // the new ltail si the gtail
+  //   && var new_ltail := st.gtail;
+
+  //   // the state transition
+  //   && m' == m.(readerState := m.readerState[ nodeId := new_st ])
+  //             .(ltails := m.ltails[nodeId := new_ltail])
+  // }
+
+
+
+  // /////////////////////////////////////////////////////////////////////////////
+  // // Append Transitions
+  // /////////////////////////////////////////////////////////////////////////////
+
+  // // pub fn append<F: FnMut(T, usize)>(&self, ops: &[T], idx: usize, mut s: F)
+
+
+  // // { AppendIdle }
+  // //   let tail = self.tail.load(Ordering::Relaxed);
+  // // { AppendAdvanceTail(ops, tail) }
+  // predicate TransitionAppendAdvanceTail(m: M, m': M, nodeId: NodeId, ops: seq<nrifc.UpdateOp>) {
+  //     && StateValid(m)
+  //     && AppendInIdle(m, nodeId)
+  //     && TailFieldValid(m)
+
+  //     // read the tail field
+  //     && var tail := m.tail.value;
+
+  //     // construct the new state
+  //     && var newst := AppendAdvanceTail(ops, tail);
+
+  //     // the state transition
+  //     && m' == m.(appendState := m.appendState[nodeId := newst])
+  // }
+  // // TODO, the case where we exec??? if tail > head + self.size - GC_FROM_HEAD {
+
+  // // { AppendAdvanceTail(ops, tail) }
+  // // self.tail.compare_exchange_weak()  // if we had another update
+  // // { AppendAdvanceTail(ops, tail) }
+  // predicate TransitionAppendWriteLogEntry(m: M, m': M, nodeId: NodeId) {
+  //     && StateValid(m)
+  //     && AppendAdvanceTail(m, nodeId)
+  //     && TailFieldValid(m)
+
+  //     // read the tail field
+  //     && var tail := m.tail.value;
+
+  //     // the old state
+  //     var st := m.appendState[nodeId];
+
+  //     // if the two tails are not equal, retry
+  //     && st.tail != tail
+
+  //     // construct the new state
+  //     && var newst := AppendAdvanceTail(ops, tail);
+
+  //     // the state transition
+  //     && m' == m.(appendState := m.appendState[nodeId := newst])
+  // }
+
+
+  // // { AppendAdvanceTail(ops, tail) }
+  // // self.tail.compare_exchange_weak()
+  // // { AppendWriteLogEntry(ops, tail, idx = 0) }
+  // predicate TransitionAppendWriteLogEntry(m: M, m': M, nodeId: NodeId) {
+  //     && StateValid(m)
+  //     && AppendInAdvanceTail(m, nodeId)
+  //     && TailFieldValid(m)
+
+  //     // read the tail field
+  //     && var tail := m.tail.value;
+
+  //     // the old state
+  //     var st := m.appendState[nodeId];
+
+  //     // the two tails must be equal
+  //     && st.tail == tail
+
+  //     // read the tail field
+  //     && var tail_new := tail + |st.ops|;
+
+  //     // construct the new state
+  //     && var newst := AppendWriteLogEntry(ops, tail, idx);
+
+  //     // the state transition
+  //     && m' == m.(appendState := m.appendState[nodeId := newst])
+  //               .(tail := Some(tail_new))
+  // }
+
+  // // { AppendWriteLogEntry(ops, tail, idx) }
+  // //   if unsafe { (*e).alivef.load(Ordering::Relaxed) == m } { m = !m; }
+  // // { AppendWriteLogEntry(ops, tail, idx) }
+  // predicate TransitionAppendWriteLogEntryOp(m: M, m': M, nodeId: NodeId) {
+  //     && StateValid(m)
+  //     && AppendInWriteLogEntryFlipMask(m, nodeId)
+
+  //     // the old state
+  //     && var st := m.appendState[nodeId];
+
+  //     // construct the new state
+  //     && var newst := AppendWriteLogEntryOp(ops, tail, idx);
+
+  //     // construct the new mask value
+  //     && var newmask := !m.lmasks[nodeId];
+
+  //     // the state transition
+  //     && m' == m.(appendState := m.appendState[nodeId := newst])
+  //               .(lmasks := m.lmasks[nodeId := newmask])
+  // }
+
+  // // { AppendWriteLogEntry(ops, tail, idx) }
+  // //   unsafe { (*e).alivef.store(m, Ordering::Release) };
+  // // { AppendWriteLogEntry(ops, tail, idx + 1) }
+  // predicate TransitionAppendWriteLogNext(m: M, m': M, nodeId: NodeId) {
+  //     && StateValid(m)
+  //     && AppendInWriteLogEntry(m, nodeId)
+
+  //     // the old state
+  //     && var st := m.appendState[nodeId];
+
+  //     // construct the new state
+  //     && var newst := AppendWriteLogEntryOp(ops, tail, idx + 1);
+
+  //     // construct the log entry
+  //     && var logentry := StoredType(st.ops[st.idx]);
+
+  //     // the state transition
+  //     && m' == m.(appendState := m.appendState[nodeId := newst])
+  //               .(slog := m.slog[st.tail + st.idx := logentry])
+  // }
+
+  // // assert idx == |ops|
+  // // { AppendWriteLogEntry(ops, tail, idx + 1) }
+  // // { AppendIdle }
+  // predicate TransitionAppendWriteLogDone(m: M, m': M, nodeId: NodeId) {
+  //     && StateValid(m)
+  //     && AppendInWriteLogEntryDone(m, nodeId)
+
+  //     // construct the new state
+  //     && var newst := AppendIdle;
+
+  //      // the state transition
+  //     && m' == m.(appendState := m.appendState[nodeId := newst])
+  // }
+
+
+
+  // /////////////////////////////////////////////////////////////////////////////
+  // // AdvanceHead Transitions
+  // /////////////////////////////////////////////////////////////////////////////
+
+  // // fn advance_head<F: FnMut(T, usize)>(&self, rid: usize, mut s: &mut F);
+
+  // // { AdvHeadIdle }
+  // //   let r = self.next.load(Ordering::Relaxed);
+  // // { AdvHeadNextLoaded(next) }
+  // predicate TransitionAdvHeadLoadNext(m: M, m': M, nodeId: NodeId) {
+  //   && StateValid(m)
+  //   && AdvHeadInIdle(m, nodeId)
+  //   && NextFieldValid(m)
+
+  //   // read the next field
+  //   && var next := m.next.value;
+
+  //   // construct the new state
+  //   && var newst := AdvHeadNextLoaded(next);
+
+  //   // update the state of the advanceHead
+  //   && m' == m.(advanceHead := m.advanceHead[ nodeId :=  newst])
+  // }
+
+  // // { AdvHeadNextLoaded(next) }
+  // //   let global_head = self.head.load(Ordering::Relaxed);
+  // // { AdvHeadHeadLoaded(next, head) }
+  // predicate TransitionAdvHeadReadHead(m: M, m': M, nodeId: NodeId) {
+  //   && StateValid(m)
+  //   && AdvHeadInNextLoaded(m, nodeId)
+  //   && HeadFieldValid(m)
+
+  //   // get the old state
+  //   && var st := m.advanceHead[nodeId];
+
+  //   // read the next field
+  //   && var head := m.head.value;
+
+  //   // construct the new state
+  //   && var newst := AdvHeadNextLoaded(st.next, head);
+
+  //   // update the state of the advanceHead
+  //   && m' == m.(advanceHead := m.advanceHead[ nodeId :=  newst])
+  // }
+
+
+  // // let f = self.tail.load(Ordering::Relaxed);
+  // // that one seems to be no-where used??
+
+  // // { AdvHeadHeadLoaded(next, head) }
+  // //   let mut min_local_tail = self.ltails[0].load(Ordering::Relaxed);
+  // // { AdvHeadMinLtail(next, head, min_local_tail, idx = 1) }
+  // predicate TransitionAdvHeadMinLTail(m: M, m': M, nodeId: NodeId) {
+  //   && StateValid(m)
+  //   && AdvHeadInReadHead(m, nodeId)
+  //   && 0 in m.localTails
+
+  //   // get the old state
+  //   && var st := m.advanceHead[nodeId];
+
+  //   // read the first local tail
+  //   && var ltail := m.localTails[0];
+
+  //   // construct the new state
+  //   && var newst := AdvHeadMinLtail(st.next, st.head, ltail, 1);
+
+  //   // update the state of the advanceHead
+  //   && m' == m.(advanceHead := m.advanceHead[ nodeId :=  newst])
+  // }
+
+
+  // // { AdvHeadMinLtail(next, head, min_local_tail, idx = 1)
+  // //   for idx in 1..r {
+  // //     let cur_local_tail = self.ltails[idx - 1].load(Ordering::Relaxed);
+  // //     if min_local_tail > cur_local_tail {
+  // //         min_local_tail = cur_local_tail
+  // //     };
+  // //   }
+  // // assert(idx == next)
+  // // { AdvHeadMinLtail(next, head, min_local_tail, idx = next)
+  // predicate TransitionAdvHeadMinLTailNext(m: M, m': M, nodeId: NodeId) {
+  //   && StateValid(m)
+  //   && AdvHeadInMinLTail(m, nodeId)
+  //   && AdvHeadMinLtailValid(m, nodeId)
+
+  //   // get the old state
+  //   && var st := m.advanceHead[nodeId];
+
+  //   // read the current local tail
+  //   && var cur_local_tail := m.localTails[st.idx];
+
+  //   // if the current local tail is smaller, update the value
+  //   && var ltail := if st.mintail > cur_local_tail then cur_local_tail else st.mintail;
+
+  //   // construct the new state
+  //   && var newst := AdvHeadMinLtail(st.next, st.head, ltail, st.idx + 1);
+
+  //   // update the state of the advanceHead
+  //   && m' == m.(advanceHead := m.advanceHead[ nodeId :=  newst])
+  // }
+
+  // // What About the exec stuff here?
+  // // { AdvHeadMinLtail(next, head, min_local_tail, idx = next)
+  // //   self.head.store(min_local_tail, Ordering::Relaxed);
+  // // { AdvHeadIdle }
+  // predicate TransitionAdvHeadIdle(m: M, m': M, nodeId: NodeId) {
+  //   && StateValid(m)
+  //   && AdvHeadInMinLTailDone(m, nodeId)
+
+  //   // get the old state
+  //   && var st := m.advanceHead[nodeId];
+
+  //   // the new head value
+  //   && var new_head := st.mintail;
+
+  //   // construct the new state
+  //   && var newst := AdvHeadIdle;
+
+  //   // update the state of the advanceHead
+  //   && m' == m.(advanceHead := m.advanceHead[ nodeId :=  newst])
+  //             .(head := Some(new_head))
+  // }
 
 }
